Wait-only broadcast restriction

models.dfy
@@ -1,24 +1,103 @@
 module Models {
 
-  type State(==)
-  type Message(==)
-
+  // --------------------------------------------------
+  // Types
+  // --------------------------------------------------
+  type State(==,!new)
+  type Message(==,!new)
+  
   datatype Action =
     | Send(m: Message)
     | Recv(m: Message)
 
+  datatype Transition = Transition(from: State, message: Action, target: State)
+
+
+  predicate IsRecv(a: Action) {
+    match a
+      case Recv(_) => true
+      case Send(_) => false
+  }
+
+  predicate IsSend(a: Action) {
+    match a
+      case Recv(_) => false
+      case Send(_) => true
+  }
+
+  // --------------------------------------------------
+  // Process type
+  // --------------------------------------------------
   class Proc {
     var Q: set<State>
     var qinit: State
-    var delta: set<(State, Action, State)>
+    var delta: set<Transition>
 
-    constructor(states: set<State>, q0: State, d: set<(State, Action, State)>)
+    constructor(q0: State, states: set<State>, d: set<Transition>)
       requires q0 in states
-      requires forall t :: t in d ==> t.0 in states && t.2 in states
     {
-      Q := states;
       qinit := q0;
+      Q := states;
       delta := d;
+    }
+  }
+
+  // --------------------------------------------------
+  // Wait-Only predicates
+  // --------------------------------------------------
+  predicate IsActive(p: Proc, q: State)
+    requires q in p.Q
+    reads p
+  {
+    forall t :: t in p.delta && t.from == q ==> !IsRecv(t.message)
+  }
+
+  predicate IsWaiting(p: Proc, q: State)
+    requires q in p.Q
+    reads p
+  {
+    exists t2 :: t2 in p.delta && t2.from == q && IsRecv(t2.message) && forall t :: t in p.delta && t.from == q ==> !IsSend(t.message)
+  }
+
+  predicate WaitOnly(p: Proc)
+    reads p
+  {
+    forall q :: q in p.Q ==> IsActive(p, q) || IsWaiting(p, q)
+  }
+
+  method ComputeActiveStates(p: Proc) returns  (states: set<State>)
+    requires WaitOnly(p)
+    ensures forall q :: q in states && q in p.Q ==> IsActive(p, q) 
+  {
+    states := {};
+    var checked := p.Q;
+    while (checked != {})
+      invariant forall q :: q in states && q in p.Q ==> IsActive(p, q)
+      decreases checked
+    {
+      var q :| q in checked;
+      if (IsActive(p, q)){
+        states := states + { q };
+      }
+      checked := checked - { q };
+    }
+  }
+
+  method ComputeWaitingStates(p: Proc) returns  (states: set<State>)
+    requires WaitOnly(p)
+    ensures forall q :: q in states && q in p.Q ==> IsWaiting(p, q)
+  {
+    states := {};
+    var checked := p.Q;
+    while (checked != {})
+      invariant forall q :: q in states && q in p.Q ==> IsWaiting(p, q)
+      decreases checked
+    {
+      var q :| q in checked;
+      if (IsWaiting(p, q)){
+        states := states + { q };
+      }
+      checked := checked - { q };
     }
   }
 }
